theories/case_studies/counter/counter_spec.v
@@ -31,12 +31,12 @@ Section Counter.
   Proof.
     intros * Htemporaries_W0 Hrevoked_W3 Hrelated_pub_W1_W2.
 
-    destruct W0 as [ [W0_std W0_cus] W0_seals],
-               W2 as [ [W2_std W2_cus] W2_seals]; cbn.
+    destruct W0 as [ [ [W0_std W0_cus] W0_seals] W_heap0 ],
+               W2 as [ [ [W2_std W2_cus] W2_seals] W_heap2 ]; cbn.
     destruct Hrelated_pub_W1_W2 as (HW1_W2_std & HW1_W2_cus & HW1_W2_seals).
     split;[|split];cbn; cycle 1.
     { eapply related_sts_pub_trans; eauto; eapply related_sts_pub_refl. }
-    { eapply related_sts_seals_trans; eauto; eapply related_sts_seals_std_refl. }
+    { exact HW1_W2_seals. }
     destruct HW1_W2_std as [HW1_W2_std_dom HW1_W2_std_t].
     cbn in *.
     split.
@@ -54,7 +54,7 @@ Section Counter.
         intro Hcontra; apply H in Hcontra. by rewrite Ha0 in Hcontra.
       }
       apply revoke_lookup_Perm in Ha0.
-      assert (std (revoke ((W0_std, W0_cus, W0_seals))) !! a = Some Permanent) as Ha0' by done.
+      assert (std (revoke ((W0_std, W0_cus, W0_seals, W_heap0))) !! a = Some Permanent) as Ha0' by done.
       rewrite -(std_sta_update_multiple_lookup_same_i _ (finz.seq_between (csp_b ^+ 4)%a csp_e) Temporary)
         in Ha0'.
       2: {
@@ -78,9 +78,9 @@ Section Counter.
       assert (a ∈ l ++ finz.seq_between csp_b csp_e) as Ha_in.
       { destruct (Htemporaries_W0 a) as [? _]; by apply Htemporaries_W0. }
       apply revoke_lookup_Monotemp in Ha0.
-      assert (std (revoke ((W0_std, W0_cus, W0_seals))) !! a = Some Revoked) as Ha0' by done.
+      assert (std (revoke ((W0_std, W0_cus, W0_seals, W_heap0))) !! a = Some Revoked) as Ha0' by done.
       assert (
-          std ((std_update_multiple (revoke (W0_std, W0_cus, W0_seals)) (finz.seq_between (csp_b ^+ 4)%a csp_e)
+          std ((std_update_multiple (revoke (W0_std, W0_cus, W0_seals, W_heap0)) (finz.seq_between (csp_b ^+ 4)%a csp_e)
                   Temporary)) !! a =
           Some (if (decide (a ∈ (finz.seq_between (csp_b ^+ 4)%a csp_e)))
                 then Temporary
