theories/case_studies/stack_object/stack_object_spec_repair.v
@@ -259,9 +259,9 @@ Section Stack_Object_Return_Repair.
           apply elem_of_finz_seq_between.
           solve_addr+Hx Hfresh Hnext Hcsp_b_ret Hret_csp_e Hret_add.
       }
-      destruct W4 as [ [W4std W4cus] W4seals]; cbn.
+      destruct W4 as [ [ [W4std W4cus] W4seals] W_heap4 ]; cbn.
       split; [|split];
-        [|apply related_sts_pub_refl|apply related_sts_seals_std_refl]; cbn.
+        [|apply related_sts_pub_refl|split; [apply related_sts_seals_std_refl|apply related_sts_heap_std_refl] ]; cbn.
       split.
       - setoid_rewrite <- close_list_dom_eq.
         setoid_rewrite <- revoke_dom_eq. done.
@@ -291,8 +291,8 @@ Section Stack_Object_Return_Repair.
         - apply elem_of_app; left. subst closing_revoked.
           by apply elem_of_app; left.
         - by apply elem_of_app; right. }
-      destruct W0 as [ [W0std W0cus] W0seals].
-      destruct W4 as [ [W4std W4cus] W4seals]. cbn in *.
+      destruct W0 as [ [ [W0std W0cus] W0seals] W_heap0 ].
+      destruct W4 as [ [ [W4std W4cus] W4seals] W_heap4 ]. cbn in *.
       split; [|split]; cbn; cycle 1.
       - destruct Hpriv as (_ & Hcus03 & _).
         destruct Hpub as (_ & Hcus34 & _).
@@ -300,11 +300,11 @@ Section Stack_Object_Return_Repair.
         cbn in *.
         eapply related_sts_pub_trans; eauto.
         apply related_sts_pub_refl.
-      - destruct Hpriv as (_ & _ & Hseals03).
-        destruct Hpub as (_ & _ & Hseals34).
-        clear -Hseals03 Hseals34.
+      - destruct Hpriv as (_ & _ & Hseals03 & Hheap03).
+        destruct Hpub as (_ & _ & Hseals34 & Hheap34).
+        clear -Hseals03 Hseals34 Hheap03 Hheap34.
         cbn in *.
-        eapply related_sts_seals_trans; eauto.
+        split; [eapply related_sts_seals_trans|eapply related_sts_heap_std_trans]; eauto.
       - split.
         + destruct Hpriv as [ [Hdom03 _] _].
           destruct Hpub as [ [Hdom34 _] _].
@@ -318,7 +318,7 @@ Section Stack_Object_Return_Repair.
             specialize (Hinitial_W5 x Hx_close).
             rewrite close_list_std_sta_revoked in Hx5; auto.
             simplify_eq; apply rtc_refl.
-          * assert (std (W4std, W4cus, W4seals) !! x = Some Permanent)
+          * assert (std (W4std, W4cus, W4seals, W_heap4) !! x = Some Permanent)
               as Hx4.
             { eapply region_state_priv_perm.
               - eapply related_sts_priv_pub_trans_world; eauto.
