theories/case_studies/vae/vae_helper.v
@@ -116,7 +116,7 @@ Section VAE_helper.
     intros Hloc Hrel.
     rewrite /related_sts_priv_world /=.
     split; first apply related_sts_std_priv_refl.
-    split; last apply related_sts_seals_std_refl.
+    split; last (split; [apply related_sts_seals_std_refl|apply related_sts_heap_std_refl]).
     split; [set_solver|split;[set_solver|] ].
     intros d rpub rpriv rpub' rpriv' Hr Hr'; simplify_eq.
     repeat (split; first done).
@@ -138,7 +138,7 @@ Section VAE_helper.
     intros Hloc Hrel.
     rewrite /related_sts_pub_world /=.
     split; first apply related_sts_std_pub_refl.
-    split; last apply related_sts_seals_std_refl.
+    split; last (split; [apply related_sts_seals_std_refl|apply related_sts_heap_std_refl]).
     split; [set_solver|split;[set_solver|] ].
     intros d rpub rpriv rpub' rpriv' Hr Hr'; simplify_eq.
     repeat (split; first done).
@@ -261,9 +261,9 @@ Section VAE_helper.
     }
 
     split; [|split]; cbn; cycle 1.
-    - destruct W0 as [ [W0_std [W0_loc W0_rel] ] W0_seals],
-          W3 as [ [W3_std [W3_loc W3_rel] ] W3_seals],
-          W6 as [ [W6_std [W6_loc W6_rel] ] W6_seals]; cbn.
+    - destruct W0 as [ [ [W0_std [W0_loc W0_rel] ] W0_seals] W_heap0 ],
+          W3 as [ [ [W3_std [W3_loc W3_rel] ] W3_seals] W_heap3 ],
+          W6 as [ [ [W6_std [W6_loc W6_rel] ] W6_seals] W_heap6 ]; cbn.
       destruct Hrelated_pub_W2_W3 as
         (HW2_W3_std & HW2_W3_cus & HW2_W3_seals).
       destruct Hrelated_pub_W5_W6 as
