theories/model/heap_allocator.v
@@ -1,0 +1,49 @@
+From griotte Require Export heap_std.
+From griotte.allocator Require Import allocator_preamble.
+
+Definition alloc_object_cell_state (s : AllocObjectStatus) : AllocState :=
+  match s with
+  | AllocObjectLive => Live
+  | AllocObjectQuarantined => Quarantined
+  end.
+
+(** Agreement at allocator operation boundaries. Headers and free cells are
+    outside object payloads. During trusted painting, the per-cell states may
+    temporarily disagree with the indivisible logical object transition. *)
+Definition heap_std_allocator_agree
+  (W_heap : Heap) (allocations : list allocator_header_entry)
+  (alloc_map : gmap Addr AllocState) : Prop :=
+  heap_wf W_heap /\
+  alloc_object_end <$> W_heap = fst <$> list_to_map allocations /\
+  ∀ b o a, W_heap !! b = Some o -> alloc_object_contains b o a ->
+    alloc_map !! a = Some (alloc_object_cell_state (alloc_object_status o)).
+
+Lemma heap_std_allocator_agree_lookup W_heap allocations alloc_map a b o :
+  heap_std_allocator_agree W_heap allocations alloc_map ->
+  heap_lookup_addr W_heap a = Some (b,o) ->
+  alloc_map !! a = Some (alloc_object_cell_state (alloc_object_status o)).
+Proof.
+  intros (_ & _ & Hcells) Hfind.
+  apply heap_lookup_addr_sound in Hfind as [Hb Ha]. eauto.
+Qed.
+
+Lemma heap_std_allocator_agree_bounds W_heap allocations alloc_map b o :
+  heap_std_allocator_agree W_heap allocations alloc_map ->
+  W_heap !! b = Some o ->
+  ∃ reserved : Z, (list_to_map allocations : gmap Addr (Addr * Z)) !! b = Some (alloc_object_end o, reserved).
+Proof.
+  intros (_ & Hbounds & _) Hb.
+  assert (((alloc_object_end <$> W_heap) : gmap Addr Addr) !! b =
+    ((fst <$> list_to_map allocations) : gmap Addr Addr) !! b) as Hlookup
+    by (rewrite Hbounds; reflexivity).
+  rewrite !lookup_fmap Hb /= in Hlookup.
+  symmetry in Hlookup. apply fmap_Some in Hlookup as ([e r] & He & Heq).
+  cbn in Heq. subst e. eauto.
+Qed.
+
+Lemma heap_std_allocator_agree_empty alloc_map :
+  heap_std_allocator_agree ∅ [] alloc_map.
+Proof.
+  split; first apply heap_wf_empty. split; first by rewrite /= !fmap_empty.
+  intros b o a Hb. rewrite lookup_empty in Hb. discriminate.
+Qed.
