theories/model/heap_std.v
@@ -1,0 +1,292 @@
+From stdpp Require Import gmap list.
+From griotte Require Export addresses.
+
+(** Allocation objects describe payloads, not allocator headers or free cells.
+    The original base is the identity and is never reused. The map key agrees
+    with the base recorded in the object. *)
+Inductive AllocObjectStatus := AllocObjectLive | AllocObjectQuarantined.
+
+Global Instance alloc_object_status_eq_dec : EqDecision AllocObjectStatus.
+Proof. solve_decision. Defined.
+
+Record AllocObject := MkAllocObject {
+  alloc_object_base : Addr;
+  alloc_object_end : Addr;
+  alloc_object_status : AllocObjectStatus;
+}.
+
+Global Instance alloc_object_eq_dec : EqDecision AllocObject.
+Proof. solve_decision. Defined.
+
+Definition Heap := gmap Addr AllocObject.
+
+Definition alloc_object_contains (b : Addr) (o : AllocObject) (a : Addr) : Prop :=
+  (b <= a < alloc_object_end o)%a.
+
+Global Instance alloc_object_contains_dec b o a :
+  Decision (alloc_object_contains b o a).
+Proof. unfold alloc_object_contains. apply _. Defined.
+
+Definition heap_entry_valid (W_heap : Heap) (b : Addr) (o : AllocObject) : Prop :=
+  b = alloc_object_base o /\ (b < alloc_object_end o)%a /\
+  ∀ b' o' a, W_heap !! b' = Some o' ->
+    alloc_object_contains b o a -> alloc_object_contains b' o' a -> b = b'.
+
+Definition heap_wf (W_heap : Heap) : Prop :=
+  ∀ b o, W_heap !! b = Some o -> heap_entry_valid W_heap b o.
+
+Definition alloc_object_future (o o' : AllocObject) : Prop :=
+  alloc_object_base o = alloc_object_base o' /\
+  alloc_object_end o = alloc_object_end o' /\
+  (alloc_object_status o = AllocObjectQuarantined ->
+   alloc_object_status o' = AllocObjectQuarantined).
+
+(** Both public and private futures use this relation. A fresh object may
+    already be quarantined in a future reached by several operations. *)
+Definition related_sts_heap_std (W_heap W_heap' : Heap) : Prop :=
+  (∀ b o, W_heap !! b = Some o ->
+    ∃ o', W_heap' !! b = Some o' /\ alloc_object_future o o') /\
+  (∀ b o, W_heap !! b = None -> W_heap' !! b = Some o -> heap_entry_valid W_heap' b o).
+
+Lemma heap_wf_empty : heap_wf ∅.
+Proof. intros b o. rewrite lookup_empty. discriminate. Qed.
+
+Lemma alloc_object_future_refl o : alloc_object_future o o.
+Proof. repeat split; auto. Qed.
+
+Lemma alloc_object_future_trans o1 o2 o3 :
+  alloc_object_future o1 o2 -> alloc_object_future o2 o3 -> alloc_object_future o1 o3.
+Proof. intros (Hb12 & He12 & Hs12) (Hb23 & He23 & Hs23). split; [congruence|]. split; [congruence|auto]. Qed.
+
+Lemma related_sts_heap_std_refl W_heap : related_sts_heap_std W_heap W_heap.
+Proof.
+  split.
+  - intros b o Hb. exists o. split; auto using alloc_object_future_refl.
+  - intros b o Hb Hb'. congruence.
+Qed.
+
+Lemma heap_entry_valid_future W_heap W_heap' b o o' :
+  related_sts_heap_std W_heap W_heap' -> W_heap !! b = Some o ->
+  W_heap' !! b = Some o' -> heap_entry_valid W_heap b o -> heap_entry_valid W_heap' b o'.
+Proof.
+  intros [Hkeep Hnew] Hb Hb' (Hbase & Hnonempty & Hdisj).
+  destruct (Hkeep b o Hb) as (ox & Hox & Hbase' & He & Hs).
+  simplify_eq. split; first congruence. split; first by rewrite -He.
+  intros c oc a Hc Ha Hca.
+  destruct (W_heap !! c) as [old|] eqn:Hc0.
+  - destruct (Hkeep c old Hc0) as (oc' & Hoc' & Hbc & Hec & Hsc).
+    simplify_eq. eapply Hdisj; eauto.
+    + unfold alloc_object_contains in *. by rewrite He.
+    + unfold alloc_object_contains in *. by rewrite Hec.
+  - destruct (Hnew c oc Hc0 Hc) as (_ & _ & Hfresh).
+    symmetry. eapply Hfresh; eauto.
+Qed.
+
+Lemma related_sts_heap_std_trans W_heap1 W_heap2 W_heap3 :
+  related_sts_heap_std W_heap1 W_heap2 -> related_sts_heap_std W_heap2 W_heap3 ->
+  related_sts_heap_std W_heap1 W_heap3.
+Proof.
+  intros H12 H23. destruct H12 as [Hkeep12 Hnew12].
+  destruct H23 as [Hkeep23 Hnew23]. split.
+  - intros b o Hb. destruct (Hkeep12 b o Hb) as (o2 & Hb2 & Ho2).
+    destruct (Hkeep23 b o2 Hb2) as (o3 & Hb3 & Ho3).
+    exists o3. split; eauto using alloc_object_future_trans.
+  - intros b o Hb Hb3. destruct (W_heap2 !! b) as [o2|] eqn:Hb2.
+    + eapply heap_entry_valid_future; eauto. split; assumption.
+    + eauto.
+Qed.
+
+Lemma related_sts_heap_std_wf W_heap W_heap' :
+  related_sts_heap_std W_heap W_heap' -> heap_wf W_heap -> heap_wf W_heap'.
+Proof.
+  intros Hrel Hwf b o Hb. destruct (W_heap !! b) as [old|] eqn:Hb0.
+  - eapply heap_entry_valid_future; eauto.
+  - apply (proj2 Hrel b o Hb0 Hb).
+Qed.
+
+Lemma related_sts_heap_std_empty W_heap :
+  heap_wf W_heap -> related_sts_heap_std ∅ W_heap.
+Proof.
+  intros Hwf. split.
+  - intros b o Hb. rewrite lookup_empty in Hb. discriminate.
+  - intros b o _ Hb. by apply Hwf.
+Qed.
+
+Lemma related_sts_heap_std_dom W_heap W_heap' :
+  related_sts_heap_std W_heap W_heap' -> dom W_heap ⊆ dom W_heap'.
+Proof.
+  intros [Hkeep _] b. rewrite !elem_of_dom.
+  intros [o Hb]. destruct (Hkeep b o Hb) as (o' & Hb' & _). eauto.
+Qed.
+
+Lemma related_sts_heap_std_quarantined W_heap W_heap' b e :
+  related_sts_heap_std W_heap W_heap' -> W_heap !! b = Some (MkAllocObject b e AllocObjectQuarantined) ->
+  W_heap' !! b = Some (MkAllocObject b e AllocObjectQuarantined).
+Proof.
+  intros [Hkeep _] Hb. destruct (Hkeep _ _ Hb) as ([b' e' s'] & Hb' & Hb_eq & He & Hs).
+  cbn in *. specialize (Hs eq_refl). by subst.
+Qed.
+
+Definition heap_lookup_addr (W_heap : Heap) (a : Addr) : option (Addr * AllocObject) :=
+  snd <$> list_find (λ bo, alloc_object_contains bo.1 bo.2 a) (map_to_list W_heap).
+
+Lemma heap_lookup_addr_sound W_heap a b o :
+  heap_lookup_addr W_heap a = Some (b,o) ->
+  W_heap !! b = Some o /\ alloc_object_contains b o a.
+Proof.
+  rewrite /heap_lookup_addr. intros Hfind.
+  apply fmap_Some in Hfind as ([i [b' o']] & Hfind & Heq).
+  cbn in Heq. simplify_eq. apply list_find_Some in Hfind as [Hlookup [Ha _]].
+  split; last done. apply elem_of_map_to_list. eapply list_elem_of_lookup_2; eauto.
+Qed.
+
+Lemma heap_lookup_addr_complete W_heap a b o :
+  heap_wf W_heap -> W_heap !! b = Some o -> alloc_object_contains b o a ->
+  heap_lookup_addr W_heap a = Some (b,o).
+Proof.
+  intros Hwf Hb Ha.
+  destruct (list_find_elem_of (λ bo : Addr * AllocObject,
+    alloc_object_contains bo.1 bo.2 a) (map_to_list W_heap) (b,o))
+    as [[i [b' o']] Hfind]; [by apply elem_of_map_to_list|exact Ha|].
+  rewrite /heap_lookup_addr Hfind /=.
+  apply list_find_Some in Hfind as [Hlookup [Ha' _]].
+  assert (W_heap !! b' = Some o') as Hb'.
+  { apply elem_of_map_to_list. eapply list_elem_of_lookup_2; eauto. }
+  destruct (Hwf b o Hb) as (_ & _ & Hunique).
+  assert (b = b') by (eapply Hunique; eauto). simplify_eq. done.
+Qed.
+
+Lemma heap_lookup_addr_none W_heap a :
+  heap_wf W_heap ->
+  (heap_lookup_addr W_heap a = None <-> ∀ b o, W_heap !! b = Some o -> ~ alloc_object_contains b o a).
+Proof.
+  intros Hwf. split.
+  - intros Hnone b o Hb Ha. rewrite (heap_lookup_addr_complete W_heap a b o Hwf Hb Ha) in Hnone.
+    discriminate.
+  - intros Hnone. destruct (heap_lookup_addr W_heap a) as [[b o]|] eqn:Hfind; last done.
+    apply heap_lookup_addr_sound in Hfind as [Hb Ha]. exfalso. exact (Hnone b o Hb Ha).
+Qed.
+
+Lemma heap_lookup_addr_future W_heap W_heap' a b o :
+  heap_wf W_heap' -> related_sts_heap_std W_heap W_heap' -> heap_lookup_addr W_heap a = Some (b,o) ->
+  ∃ o', heap_lookup_addr W_heap' a = Some (b,o') /\ alloc_object_future o o'.
+Proof.
+  intros Hwf [Hkeep _] Hfind. apply heap_lookup_addr_sound in Hfind as [Hb Ha].
+  destruct (Hkeep b o Hb) as (o' & Hb' & Ho').
+  exists o'. split; last done. apply heap_lookup_addr_complete; auto.
+  unfold alloc_object_contains in *. by rewrite -(proj1 (proj2 Ho')).
+Qed.
+
+Definition heap_allocate (W_heap : Heap) (b e : Addr) : Heap :=
+  <[b := MkAllocObject b e AllocObjectLive]> W_heap.
+
+Definition heap_fresh (W_heap : Heap) (b e : Addr) : Prop :=
+  W_heap !! b = None /\ (b < e)%a /\
+  ∀ c o a, W_heap !! c = Some o -> (b <= a < e)%a -> ~ alloc_object_contains c o a.
+
+Lemma heap_allocate_future W_heap b e :
+  heap_fresh W_heap b e -> related_sts_heap_std W_heap (heap_allocate W_heap b e).
+Proof.
+  intros [Hb [Hbe Hdisj]]. split.
+  - intros c o Hc. exists o. split; last apply alloc_object_future_refl.
+    rewrite /heap_allocate fin_maps.lookup_insert_ne; [exact Hc|intros ->; congruence].
+  - intros c o Hc Hnew. rewrite /heap_allocate in Hnew.
+    apply fin_maps.lookup_insert_Some in Hnew as [[-> <-]|[_ Hcontra]]; last by rewrite Hc in Hcontra.
+    split; first done. split; first done. intros d oc a Hc' Ha Hca.
+    rewrite /heap_allocate in Hc'.
+    apply fin_maps.lookup_insert_Some in Hc' as [[-> <-]|[_ Hc']]; first done.
+    exfalso. eapply Hdisj; eauto.
+Qed.
+
+Lemma heap_allocate_wf W_heap b e :
+  heap_wf W_heap -> heap_fresh W_heap b e -> heap_wf (heap_allocate W_heap b e).
+Proof. eauto using related_sts_heap_std_wf, heap_allocate_future. Qed.
+
+(** Adjusting the one object entry changes the status of its entire interval. *)
+Definition heap_quarantine (W_heap : Heap) (b : Addr) : Heap :=
+  alter (λ o, MkAllocObject (alloc_object_base o) (alloc_object_end o) AllocObjectQuarantined) b W_heap.
+
+Definition heap_quarantine_addr (W_heap : Heap) (a : Addr) : option Heap :=
+  (λ bo, heap_quarantine W_heap bo.1) <$> heap_lookup_addr W_heap a.
+
+Lemma heap_quarantine_lookup W_heap b o :
+  W_heap !! b = Some o ->
+  heap_quarantine W_heap b !! b = Some (MkAllocObject (alloc_object_base o) (alloc_object_end o) AllocObjectQuarantined).
+Proof. intros Hb. by rewrite /heap_quarantine fin_maps.lookup_alter_eq Hb. Qed.
+
+Lemma heap_quarantine_lookup_ne W_heap b c :
+  b ≠ c -> heap_quarantine W_heap b !! c = W_heap !! c.
+Proof. intros Hne. by rewrite /heap_quarantine fin_maps.lookup_alter_ne. Qed.
+
+Lemma heap_quarantine_future W_heap b : related_sts_heap_std W_heap (heap_quarantine W_heap b).
+Proof.
+  split.
+  - intros c o Hc. destruct (decide (b = c)) as [->|Hne].
+    + exists (MkAllocObject (alloc_object_base o) (alloc_object_end o) AllocObjectQuarantined).
+      split; first by apply heap_quarantine_lookup. repeat split; done.
+    + exists o. rewrite heap_quarantine_lookup_ne; last done.
+      split; auto using alloc_object_future_refl.
+  - intros c o Hc Hnew. destruct (decide (b = c)) as [->|Hne].
+    + rewrite /heap_quarantine fin_maps.lookup_alter_eq Hc /= in Hnew. discriminate.
+    + rewrite heap_quarantine_lookup_ne // Hc in Hnew. discriminate.
+Qed.
+
+Lemma heap_quarantine_wf W_heap b : heap_wf W_heap -> heap_wf (heap_quarantine W_heap b).
+Proof. eauto using related_sts_heap_std_wf, heap_quarantine_future. Qed.
+
+Lemma heap_quarantine_idempotent W_heap b :
+  heap_quarantine (heap_quarantine W_heap b) b = heap_quarantine W_heap b.
+Proof.
+  apply map_eq. intros c. destruct (decide (b = c)) as [->|Hne].
+  - rewrite /heap_quarantine !fin_maps.lookup_alter_eq. destruct (W_heap !! c) eqn:Hc; by rewrite Hc.
+  - by rewrite !heap_quarantine_lookup_ne.
+Qed.
+
+Lemma heap_quarantine_addr_whole_object W_heap a b o a' :
+  heap_wf W_heap -> heap_lookup_addr W_heap a = Some (b,o) ->
+  alloc_object_contains b o a' ->
+  heap_quarantine_addr W_heap a = Some (heap_quarantine W_heap b) /\
+  heap_lookup_addr (heap_quarantine W_heap b) a' =
+    Some (b, MkAllocObject (alloc_object_base o) (alloc_object_end o) AllocObjectQuarantined).
+Proof.
+  intros Hwf Hfind Ha'. split; first by rewrite /heap_quarantine_addr Hfind.
+  apply heap_lookup_addr_sound in Hfind as [Hb Ha].
+  apply heap_lookup_addr_complete; eauto using heap_quarantine_wf, heap_quarantine_lookup.
+Qed.
+
+Lemma heap_lookup_addr_base W_heap a b o :
+  heap_wf W_heap -> heap_lookup_addr W_heap a = Some (b,o) ->
+  b = alloc_object_base o.
+Proof.
+  intros Hwf Hfind. apply heap_lookup_addr_sound in Hfind as [Hb _].
+  exact (proj1 (Hwf b o Hb)).
+Qed.
+
+Lemma heap_lookup_original_base W_heap b o :
+  heap_wf W_heap -> W_heap !! b = Some o ->
+  heap_lookup_addr W_heap b = Some (b,o).
+Proof.
+  intros Hwf Hb. apply heap_lookup_addr_complete; auto.
+  destruct (Hwf b o Hb) as (_ & Hnonempty & _).
+  unfold alloc_object_contains. split; [reflexivity|exact Hnonempty].
+Qed.
+
+Lemma heap_lookup_exclusive_end W_heap b o :
+  heap_lookup_addr W_heap (alloc_object_end o) ≠ Some (b,o).
+Proof.
+  intros Hfind. apply heap_lookup_addr_sound in Hfind as [_ [_ Hlt]].
+  unfold finz.lt in Hlt. lia.
+Qed.
+
+Lemma heap_fresh_no_reuse W_heap b e o :
+  W_heap !! b = Some o -> ~ heap_fresh W_heap b e.
+Proof. intros Hb [Hnone _]. rewrite Hb in Hnone. discriminate. Qed.
+
+Lemma heap_quarantine_addr_none W_heap a :
+  heap_lookup_addr W_heap a = None -> heap_quarantine_addr W_heap a = None.
+Proof. intros Hnone. by rewrite /heap_quarantine_addr Hnone. Qed.
+
+Lemma alloc_object_no_reverse b e :
+  ~ alloc_object_future (MkAllocObject b e AllocObjectQuarantined)
+      (MkAllocObject b e AllocObjectLive).
+Proof. intros (_ & _ & Hs). discriminate (Hs eq_refl). Qed.
