theories/model/world_ghost_theory.v
@@ -1077,14 +1077,14 @@ Section world_interp_Pre.
 
   Lemma world_interp_init (oset : gset OType) :
     ⊢ |==> (∃ (relg: relGS Σ) (stsg : STSG Addr region_type OType Word Σ) (sstoreg : sealStoreG Σ),
-            ([∗ set] C ∈ CNames, world_interp (∅, (∅,∅), ∅) C) ∗
+            heap_std_auth ∅ ∗ ([∗ set] C ∈ CNames, world_interp (∅, (∅,∅), ∅, ∅) C) ∗
             ([∗ set] o ∈ oset, can_alloc_pred o)).
   Proof.
-    iMod (gen_sts_init) as (stsg) "Hsts". (*XX*)
+    iMod (gen_sts_init) as (stsg) "[Hheap Hsts]".
     iMod (rel_init) as (relg) "HRELS".
     iMod (seal_store_init) as (sstoreg) "Hseals".
-    iExists relg, stsg, sstoreg; iFrame "Hseals".
-    set (Wempty := (∅, (∅,∅), ∅)).
+    iExists relg, stsg, sstoreg; iFrame "Hheap Hseals".
+    set (Wempty := (∅, (∅,∅), ∅, ∅)).
     iAssert ([∗ set] C ∈ CNames, region Wempty C)%I with "[HRELS]" as "Hr".
     { iApply (big_sepS_impl with "HRELS").
       iModIntro; iIntros (C HC) "HRELS".
